Reformatting BT_Table
Now matches CURSOR_TABLE, but with mostly stub definitions and admitted
proofs.

model/BTreesModule.v
@@ -48,19 +48,54 @@ End CURSOR_TABLE.
 
 (* NOT up to date *)
 Module BT_Table <: CURSOR_TABLE.
+ Definition b : nat. Admitted.
+ Definition key := Z.
+
  Definition V := Type.
  Definition table := forest V.
  Definition cursor := BTrees.cursor V.
- Definition b : nat. Admitted.
- Definition key := Z.
  Definition empty_t : table := (BTrees.nil V).
- Definition empty_c : cursor := [].
- Definition get (k: key) (m: table) : option V := lookup V b k m.
- Definition set (k: key) (v: V) (m: table) : table := insert V b k v (make_cursor V b k m []).
- Theorem gempty: forall k, get k empty_t = None.
-   Proof. intros. unfold get. unfold empty. Admitted.
- Theorem gss: forall k v t,  get k (set k v t) = Some v.
-   Proof. Admitted.
- Theorem gso: forall j k v t, j<>k -> get j (set k v t) = get j t.
-   Proof. Admitted.
+
+ Definition make_cursor (k: key) (m: table) : cursor := BTrees.make_cursor V b k m [].
+ Definition get_key (c: cursor) : option key := None. (* complete this *)
+ Definition get (c: cursor) : option V := None. (* complete this *) (* lookup V b k m. *)
+ Definition set (c: cursor) (v: V) : table := empty_t. (* complete this *)
+ Definition insert (c: cursor) (k: key) (v: V) : table := insert V b k v c.
+ Definition next (c: cursor) : cursor := []. (* complete this *)
+ Definition prev (c: cursor) : cursor := []. (* complete this *)
+ Definition first_cursor (m: table) : cursor := []. (* complete this *)
+ Definition last_cursor (m: table) : cursor := []. (* complete this *)
+
+ Definition abs_rel (m: table) (c: cursor) : Prop := True. (* complete this *)
+ Definition key_rel (k: key) (c: cursor) : Prop := True. (* complete this *)
+
+ Theorem make_cursor_rel: forall t k,
+   abs_rel t (make_cursor k t).
+ Proof. Admitted.
+
+ Theorem glast: forall t,        (* get-last *)
+   get (last_cursor t) = None.
+ Proof. Admitted.
+ Theorem gss: forall k v c,      (* get-set-same *)
+   get_key c = Some k -> get (make_cursor k (set c v)) = Some v.
+ Proof. Admitted.
+ Theorem gso: forall j v c t,    (* get-set-other *)
+   abs_rel t c -> ~ key_rel j c -> get (make_cursor j (set c v)) = get (make_cursor j t).
+ Proof. Admitted.
+ Theorem gis: forall k v c,      (* get-insert-same *)
+   key_rel k c -> get (make_cursor k (insert c k v)) = Some v.
+ Proof. Admitted.
+ Theorem gio: forall j k v c t,    (* get-insert-other *)
+   key_rel k c -> ~ key_rel j c -> abs_rel t c -> get (make_cursor j (insert c k v)) = get (make_cursor j t).
+ Proof. Admitted.
+
+ Theorem next_prev: forall c t,
+       abs_rel t c -> ~ (c = last_cursor t) -> prev (next c) = c.
+ Proof. Admitted.
+ Theorem prev_next: forall c t,
+       abs_rel t c -> ~ (c = first_cursor t) -> next (prev c) = c.
+ Proof. Admitted.
+ Theorem cursor_order: forall c k1 k2, (* I don't love the use of lt_key here *)
+       get_key c = Some k1 -> get_key (next c) = Some k2 -> lt_key k1 k2 = true.
+ Proof. Admitted.
 End BT_Table.
